Batteries.lean
@@ -21,7 +21,6 @@ public import Batteries.Control.Monad
 public import Batteries.Control.Nondet.Basic
 public import Batteries.Control.OptionT
 public import Batteries.Data.Array
-public import Batteries.Data.Bool
 public import Batteries.Data.AssocList
 public import Batteries.Data.BinaryHeap
 public import Batteries.Data.BinomialHeap
